share/steel/examples/pulse/dice/common/HashTable.fsti
@@ -1,0 +1,19 @@
+module HashTable
+open Pulse.Main
+open Pulse.Steel.Wrapper
+open FStar.Ghost
+open Steel.ST.Util
+open Steel.FractionalPermission
+module A = Steel.ST.Array
+module US = FStar.SizeT
+module U32 = FStar.UInt32
+
+val session_table_len : US.t
+val context_table_len : US.t
+
+val new_table (_:unit) 
+  : stt (A.array U32.t) 
+     (requires emp)
+     (ensures fun a ->
+        A.pts_to a full_perm (Seq.create (US.v session_table_len) 0ul) `star`
+        pure (A.length a == US.v session_table_len /\ A.is_full_array a))
